initial spec for ttbr0 page table and modified pages; not connected to anything else yet

verified/ARMdef.dfy
@@ -17,11 +17,11 @@ datatype SReg = cpsr | spsr(m:mode) | scr | ttbr0
 // The abstract representation should be used for reasoning about the status of
 // the processor and the concrete representation should be used only for
 // ensuring that the correct values are stored/returned by instructions
-datatype config = Config(cpsr:PSR, spsr:map<mode,PSR>, scr:SCR, ttbr0:int, 
+datatype config = Config(cpsr:PSR, spsr:map<mode,PSR>, scr:SCR, ttbr0:TTBR, 
     ex:exception)
 datatype PSR  = PSR(m:mode)           // See B1.3.3
 datatype SCR  = SCR(ns:world)         // See B4.1.129
-//       TTBR0                           See B4.1.154
+datatype TTBR = TTBR(ptbase:mem)      // See B4.1.154
 
 type mem = int
 datatype operand = OConst(n:int) 
@@ -101,6 +101,12 @@ function decode_scr(v:int) : SCR
     requires isUInt32(v)
     { SCR(if(and32(v, 1) == 1) then NotSecure else Secure) }
 
+function decode_ttbr(v:int): TTBR
+    requires isUInt32(v)
+    ensures PageAligned(decode_ttbr(v).ptbase)
+    // assuming 4k alignment, n == 2 / x == 12
+    { MaskWithSizeIsAligned(v, 0x1000); TTBR(and32(v, 0xffff_f000)) }
+
 function decode_sreg(s:state, sr:SReg, v:int) : config
     requires ValidConfig(s.conf)
     requires ValidSpecialOperand(s, OSReg(sr))
@@ -110,7 +116,7 @@ function decode_sreg(s:state, sr:SReg, v:int) : config
 {
     reveal_ValidConfig();
     match sr
-        case ttbr0 => s.conf.(ttbr0 := v)
+        case ttbr0 => s.conf.(ttbr0 := decode_ttbr(v))
         case cpsr  => s.conf.(cpsr := decode_psr(v))
         case spsr(m)  => 
             assert m != User;
@@ -267,7 +273,7 @@ predicate {:opaque} ValidRegState(regs:map<ARMReg, int>)
 
 predicate {:opaque} ValidConfig(c:config)
 {
-    isUInt32(c.ttbr0) &&
+    isUInt32(c.ttbr0.ptbase) && PageAligned(c.ttbr0.ptbase) &&
     User !in c.spsr &&
     (forall m:mode :: m != User ==> m in c.spsr )
 }
@@ -385,6 +391,178 @@ function {:axiom} TheGlobalDecls(): globaldecls
     ensures ValidGlobalDecls(TheGlobalDecls());
 
 //-----------------------------------------------------------------------------
+// Model of page tables for userspace execution
+//-----------------------------------------------------------------------------
+
+function method PAGESIZE():int { 0x1000 }
+
+predicate PageAligned(addr:mem)
+    ensures PageAligned(addr) ==> WordAligned(addr)
+{
+    // XXX: help out poor dafny
+    assert addr % 0x1000 == 0 ==> addr % 4 == 0;
+    addr % 0x1000 == 0
+}
+
+// We model a trivial memory map (for our own code and page tables)
+// with a flat 1:1 mapping of virtual to physical addresses.
+function {:axiom} PhysBase(): mem
+    ensures PageAligned(PhysBase());
+
+// Our model of page tables is also very abstract, because it just needs to encode
+// which pages are mapped and their permissions
+type AbsPTable = seq<Maybe<AbsL2PTable>>
+type AbsL2PTable = seq<Maybe<AbsPTE>>
+datatype AbsPTE = AbsPTE(phys: mem, write: bool, exec: bool)
+
+function method ARM_L1PTES(): int { 1024 }
+function ARM_L1PTABLE_BYTES(): int { ARM_L1PTES() * BytesPerWord() }
+function method ARM_L2PTES(): int { 256 }
+function ARM_L2PTABLE_BYTES(): int { ARM_L2PTES() * BytesPerWord() }
+
+predicate WellformedAbsPTable(pt: AbsPTable)
+{
+    |pt| == ARM_L1PTES()
+        && forall i :: 0 <= i < |pt| && pt[i].Just? ==> WellformedAbsL2PTable(fromJust(pt[i]))
+}
+
+predicate WellformedAbsL2PTable(pt: AbsL2PTable)
+{
+    |pt| == ARM_L2PTES() &&
+        forall i :: 0 <= i < |pt| && pt[i].Just? ==> WellformedAbsPTE(fromJust(pt[i]))
+}
+
+predicate WellformedAbsPTE(pte: AbsPTE)
+{
+    PageAligned(pte.phys)
+}
+
+function ExtractAbsPageTable(s:state): Maybe<AbsPTable>
+    requires ValidState(s)
+    ensures var r := ExtractAbsPageTable(s);
+        r.Just? ==> WellformedAbsPTable(fromJust(r))
+{
+    reveal_ValidConfig();
+    var vbase := s.conf.ttbr0.ptbase + PhysBase();
+    if ValidMemRange(s.m, vbase, vbase + ARM_L1PTABLE_BYTES()) then
+        ExtractAbsL1PTable(s.m, vbase, 0)
+    else
+        Nothing
+}
+
+function WritablePagesInTable(pt:AbsPTable): set<mem>
+    requires WellformedAbsPTable(pt)
+    ensures forall m :: m in WritablePagesInTable(pt) ==> PageAligned(m)
+{
+    (set i, j | 0 <= i < |pt| && pt[i].Just? && 0 <= j < |fromJust(pt[i])|
+        && fromJust(pt[i])[j].Just? && fromJust(fromJust(pt[i])[j]).write
+        :: fromJust(fromJust(pt[i])[j]).phys + PhysBase())
+}
+
+function ExtractAbsL1PTable(m:memstate, vbase:mem, index:nat): Maybe<AbsPTable>
+    requires ValidMemState(m)
+    requires WordAligned(vbase)
+        && ValidMemRange(m, vbase, vbase + ARM_L1PTABLE_BYTES())
+    requires 0 <= index <= ARM_L1PTES()
+    ensures var r := ExtractAbsL1PTable(m, vbase, index);
+        r.Just? ==> |fromJust(r)| == ARM_L1PTES() - index
+            && forall i :: 0 <= i < |fromJust(r)| && fromJust(r)[i].Just?
+                ==> WellformedAbsL2PTable(fromJust(fromJust(r)[i]))
+    decreases ARM_L1PTES() - index
+{
+    // stopping condition
+    if index == ARM_L1PTES() then Just([]) else
+    // extract L1 PTE and check its validity
+    var pte' := ExtractAbsL1PTE(MemContents(m, vbase + index * BytesPerWord()));
+    if pte'.Nothing? then Nothing else
+    var pte := fromJust(pte');
+    // extract the rest (recursive step)
+    var rest := ExtractAbsL1PTable(m, vbase, index + 1);
+    if rest.Nothing? then Nothing else
+    if pte.Nothing? then
+        Just([Nothing] + fromJust(rest))
+    else
+        // check validity of mem pointed to by L1 PTE
+        var l2vbase := fromJust(pte) + PhysBase();
+        if !ValidMemRange(m, l2vbase, l2vbase + ARM_L2PTABLE_BYTES()) then Nothing
+        else
+            // extract L2 table that it points to, and check its validity
+            var l2table := ExtractAbsL2PTable(m, l2vbase, 0);
+            if l2table.Nothing? then Nothing
+            else Just([l2table] + fromJust(rest))
+}
+
+/* ARM ref B3.5.1 short descriptor format for first-level page table */
+function ExtractAbsL1PTE(pte:int): Maybe<Maybe<int>>
+    requires isUInt32(pte)
+    ensures var r := ExtractAbsL1PTE(pte);
+        r.Just? && fromJust(r).Just? ==> WordAligned(fromJust(fromJust(r)))
+{
+    // for now, we just consider secure L1 tables in domain zero
+    // (i.e., no other bits set)
+    var typebits := and32(pte, 0x3);
+    var lowbits := and32(pte, 0x3ff);
+    MaskWithSizeIsAligned(pte, 0x400);
+    var ptbase := and32(pte, 0xfffffc00);
+    // if the type is zero, it's an invalid entry, which is fine (maps nothing)
+    if typebits == 0 then Just(Nothing)
+    // otherwise, the lowbits must be 1 (it maps a page table)
+    else if lowbits == 1 then Just(Just(ptbase))
+    // anything else is invalid
+    else Nothing
+}
+
+function ExtractAbsL2PTable(m:memstate, vbase:int, index:nat): Maybe<AbsL2PTable>
+    requires ValidMemState(m)
+    requires WordAligned(vbase)
+        && ValidMemRange(m, vbase, vbase + ARM_L2PTABLE_BYTES())
+    requires 0 <= index <= ARM_L2PTES()
+    ensures var r := ExtractAbsL2PTable(m, vbase, index);
+        r.Just? ==> |fromJust(r)| == ARM_L2PTES() - index
+            && forall i :: 0 <= i < |fromJust(r)| && fromJust(r)[i].Just?
+                ==> WellformedAbsPTE(fromJust(fromJust(r)[i]))
+    decreases ARM_L2PTES() - index
+{
+    // stopping condition
+    if index == ARM_L2PTES() then Just([]) else
+    // extract PTE and check its validity
+    var pte := ExtractAbsL2PTE(MemContents(m, vbase + index * BytesPerWord()));
+    if pte.Nothing? then Nothing else
+    // extract the rest (recursive step)
+    var rest := ExtractAbsL2PTable(m, vbase, index + 1);
+    if rest.Nothing? then Nothing else
+    Just([fromJust(pte)] + fromJust(rest))
+}
+
+function ExtractAbsL2PTE(pte:int): Maybe<Maybe<AbsPTE>>
+    requires isUInt32(pte)
+    ensures var r := ExtractAbsL2PTE(pte);
+        r.Just? && fromJust(r).Just? ==> WellformedAbsPTE(fromJust(fromJust(r)))
+{
+    var typebits := and32(pte, 0x3);
+    // if the type is zero, it's an invalid entry, which is fine (maps nothing)
+    if typebits == 0 then Just(Nothing) else
+    // large pages aren't supported
+    if typebits == 1 then Nothing else
+    var lowbits := and32(pte, 0xfdfc);
+    if lowbits != ARM_L2PTE_CONST_BITS() then Nothing else
+    var exec := and32(pte, 1) == 0; // !XN bit
+    var write := and32(pte, 0x200) == 0; // !AP2 bit
+    MaskWithSizeIsAligned(pte, 0x1000);
+    var pagebase := and32(pte, 0xfffff000);
+    Just(Just(AbsPTE(pagebase, write, exec)))
+}
+
+function ARM_L2PTE_CONST_BITS(): int
+{
+    0x4 /* B */
+        + 0x30 /* AP0, AP1 */
+        + 0x140 /* TEX */
+        + 0x400 /* S */
+        + 0x800 /* NG */
+}
+
+//-----------------------------------------------------------------------------
 // Functions for bitwise operations
 //-----------------------------------------------------------------------------
 function xor32(x:int, y:int) : int  
@@ -418,6 +596,13 @@ function shl32(x:int, amount:int) : int
 function shr32(x:int, amount:int) : int 
     requires isUInt32(x) && 0 <= amount < 32;
     { int(RightShift(uint32(x), uint32(amount))) }
+
+// FIXME! replace this when Dafny gains bitvector support
+lemma {:axiom} MaskWithSizeIsAligned(x:int, s:int)
+    requires isUInt32(x) && isUInt32(s)
+    // s must be a power of two. this is a cheesy approximation for that
+    requires s == 0x1000 || s == 0x400
+    ensures and32(x, 0x1_0000_0000 - s) % s == 0
 
 //-----------------------------------------------------------------------------
 // Evaluation
